word-ram/proofs/Lax13Proofs.lean
@@ -50,6 +50,7 @@ import Lax13Proofs.Refine.Ir.Semantics
 import Lax13Proofs.Refine.Ir.Assn
 import Lax13Proofs.Refine.Ir.Wp
 import Lax13Proofs.Refine.Ir.Triples
+import Lax13Proofs.Refine.Ir.Heap
 import Lax13Proofs.Refine.Ir.Attrs
 import Lax13Proofs.Refine.Ir.SepSolver
 import Lax13Proofs.Refine.Sepref.Basic
